Added the 'drop refinement' case

AnnotatedSub.v
@@ -1,5 +1,8 @@
 Require Export SystemFR.Judgments.
 Require Export SystemFR.ReducibilityLemmas.
+Require Export SystemFR.AnnotatedSubtypeSetOps.
+Require Export SystemFR.AnnotatedSubtypeOrder.
+Require Export SystemFR.AnnotatedSubtypeRefine.
 
 Opaque reducible_values.
 
@@ -11,4 +14,43 @@ Lemma annotated_reducible_sub:
 Proof.
   unfold annotated_reducible, annotated_subtype, open_reducible, open_subtype, subtype;
     repeat step; eauto using reducible_values_exprs.
+Qed.
+
+Fixpoint drop_refinement t :=
+  match t with
+  | T_refine t1 t2 => drop_refinement t1
+  | _ => t
+  end.
+Lemma drop_refinement_wf :
+  forall t k, wf t k -> wf (drop_refinement t) k.
+Proof.
+  intros.
+  induction t; steps.
+Qed.
+Hint Resolve drop_refinement_wf: wf.
+
+Lemma drop_refinement_pfv_subset :
+  forall t tag, subset (pfv (drop_refinement t) tag) (pfv t tag).
+  intros; induction t; steps; eauto using subset_left.
+Qed.
+Hint Resolve drop_refinement_pfv_subset: sets.
+
+Lemma annotated_subtype_drop :
+  forall tvars gamma T1,
+    [[tvars; gamma ⊨ T1 <: drop_refinement T1]].
+Proof.
+  intros.
+  induction T1; steps.
+  eapply subtype_trans; eauto.
+  eapply annotated_subtype_refine2.
+  steps.
+Qed.
+
+Lemma annotated_reducible_drop:
+  forall tvars gamma t T,
+    [[ tvars; gamma ⊨ t : T ]] ->
+    [[ tvars; gamma ⊨ t : (drop_refinement T) ]].
+Proof.
+  intros.
+  eapply annotated_reducible_sub; eauto; steps; eauto using annotated_subtype_drop .
 Qed.
